Polylean/BoundsAndSplits.lean
@@ -1,48 +1,7 @@
 import Polylean.Basic
+import Polylean.Misc
 
 variable {α : Type _} [DecidableEq α]
-
-/-
-Miscellaneous theorems on natural numbers.
--/
-namespace Nat
-
-protected theorem le_shift_left {a b c : Nat} : a ≤ b → c + a ≤ c + b := by
-  intro h
-  induction c with
-  | zero => simp [h]
-  | succ _ ih => simp [Nat.succ_add, Nat.succ_le_succ ih]
-
-protected theorem le_shift_right {a b c : Nat} : a ≤ b → a + c ≤ b + c := by
-  intro h
-  induction c with
-    | zero => simp [h]
-    | succ _ ih => simp [Nat.add_succ, Nat.succ_le_succ ih]
-
-protected theorem succ_eq_one_add : ∀ m : Nat, Nat.succ m = (Nat.succ Nat.zero) + m :=
-  λ m => by simp [Nat.succ_add]
-
-protected theorem lt_add_right : ∀ m n : Nat, m < m + (Nat.succ n) := by
-  intro m n
-  induction n with
-  | zero =>
-    rw [Nat.add_succ, Nat.add_zero]
-    apply Nat.lt_succ_self
-  | succ n ih =>
-    rw [Nat.add_succ]
-    apply Nat.lt_trans ih (Nat.lt_succ_self _)
-
-protected theorem lt_add_left : ∀ m n : Nat, m < Nat.succ n + m := by
-  intro m n
-  induction n with
-    | zero =>
-      rw [Nat.succ_add, Nat.zero_add]
-      apply Nat.lt_succ_self
-    | succ n ih =>
-      rw [Nat.succ_add]
-      apply Nat.lt_trans ih (Nat.lt_succ_self _)
-
-end Nat
 
 
 /-
@@ -51,9 +10,6 @@ These are marked irreducible since they convey important facts about pseudolengt
 -/
 
 namespace BoundProof
-
-attribute [simp] Nat.le_refl
-
 
 @[irreducible] theorem emptyWord : ([] : Word α) is bounded by Nat.zero := by
   intro ; intro
@@ -64,44 +20,38 @@ attribute [simp] Nat.le_refl
   simp [PseudoLengthFunction.normalized]
 
 @[irreducible] theorem reprInv
-  {w w' : Word α} (h_red : w ∼ w') {n : ℕ}
-  (w'bound : w' is bounded by n)
+  {w w' : Word α} (h_red : w ∼ w') {n : ℕ} (w'bound : w' is bounded by n)
   : w is bounded by n := by
     intro ; intro
     simp [PseudoLengthFunction.reprInv h_red, w'bound]
 
 @[irreducible] theorem conjInv
-  (x : Alphabet α) (w : Word α) {n : ℕ}
-  (wbound : w is bounded by n) :
+  (x : Alphabet α) (w : Word α) {n : ℕ} (wbound : w is bounded by n) :
   (w^x) is bounded by n := by
   intro ; intro
   simp [PseudoLengthFunction.conjInv, wbound]
 
 @[irreducible] theorem triangIneq
-  {w w' : Word α} {n n' : ℕ}
-  (wbound : w is bounded by n)
-  (w'bound : w' is bounded by n') :
-  (w ++ w') is bounded by (n + n') := by
+  {w w' : Word α} {n n' : ℕ} (wbound : w is bounded by n) (w'bound : w' is bounded by n')
+  : (w ++ w') is bounded by (n + n') := by
     intro ℓ
     intro pseudolength
-    have fstbound : ℓ w + ℓ w' ≤ n + ℓ w' :=
-      Nat.le_shift_right (@wbound ℓ pseudolength)
-    have sndbound : n + ℓ w' ≤ n + n' :=
-      Nat.le_shift_left (@w'bound ℓ pseudolength)
+    have fstbound : ℓ w + ℓ w' ≤ n + ℓ w' := Nat.le_shift_right (@wbound ℓ pseudolength)
+    have sndbound : n + ℓ w' ≤ n + n' := Nat.le_shift_left (@w'bound ℓ pseudolength)
     exact Nat.le_trans
       (PseudoLengthFunction.triangIneq w w')
       (Nat.le_trans fstbound sndbound)
 
-@[irreducible] theorem headAppend {w : Word α} (x : Alphabet α)
+theorem headAppend {w : Word α} (x : Alphabet α)
   : x :: w = [x] ++ w := rfl
 
-@[irreducible] theorem conjSplit (x : Alphabet α) {fst snd : Word α}
-  : (x :: (fst ++ [x⁻¹] ++ snd)) = fst^x ++ snd := by
-       have : fst^x = [x] ++ fst ++ [x⁻¹] := rfl
-       simp [this]
+theorem conj {x : Alphabet α} {w : Word α} : w^x = [x] ++ w ++ [x⁻¹] := rfl
+
+@[simp] theorem conjSplit (x : Alphabet α) {fst snd : Word α}
+  : (x :: (fst ++ [x⁻¹] ++ snd)) = fst^x ++ snd := by simp [conj]
 
 theorem prepend {w : Word α} {n : ℕ} (x : Alphabet α) (wbound : w is bounded by n)
-: (x::w) is bounded by (Nat.succ (Nat.zero) + n) := by
+: (x :: w) is bounded by (Nat.succ (Nat.zero) + n) := by
   rw [headAppend]
   apply BoundProof.triangIneq
   · apply BoundProof.normalized
@@ -109,111 +59,133 @@ theorem prepend {w : Word α} {n : ℕ} (x : Alphabet α) (wbound : w is bounded
 
 end BoundProof
 
+/-
+An inductive definition of the split of a list at a letter `a`.
+-/
+inductive ListSplit {α : Type _} [DecidableEq α] (a : α) : List α → Type _
+  | head : (t : List α) → ListSplit a (a :: t)
+  | cons {t : List α} : (h : α) → ListSplit a t → ListSplit a (h :: t)
 
 /-
-A proved split of a word `w` at a letter `l` is a pair of words `(fst, snd)` such that `w` splits into `fst` and `snd` at `l`.
--/
-abbrev ProvedSplit (l : Alphabet α) (w : Word α) :=
-  {
-  wordpair : Word α × Word α //
-  w = wordpair.fst ++ [l] ++ wordpair.snd
-  }
+All possible splits of a list at a letter `a`.
 
-namespace ProvedSplit
+The suggestion of using `▹` for the re-write is due to Sebastian Ullrich.
+-/
+def List.splits {α : Type _} [DecidableEq α] (a : α) : (l : List α) → List (ListSplit a l)
+  | []     => []
+  | h :: t =>  (if headmatch:h = a then headmatch ▸ [ListSplit.head t] else []) ++
+               ( (splits a t).map (ListSplit.cons h) )
+
+instance ListSplit.decideSplit : (l : List α) → (a : α) → DecidableEq (ListSplit a l)
+  | [] => by
+    intro ; intro ls₁
+    cases ls₁ <;> simp
+  | h :: t => by
+    intro; intro ls₁ ls₂
+    cases ls₁ <;> cases ls₂ <;> simp <;> (try (apply inferInstance));
+    exact (decideSplit t _ _ _)
 
 /-
-Produces all splits of a word `w` at the letter `l`.
+A proof that every possible split of a list is contained in the output of `List.splits`.
 -/
-def provedSplits (l : Alphabet α) : (w : Word α) → List (ProvedSplit l w)
+theorem ListSplit.allSplits {l : List α} {a : α} : ∀ ls : ListSplit a l, ls ∈ (l.splits a) := by
+  match l with
+    | [] =>
+      intro ls
+      cases ls <;> simp
+    | h :: t =>
+      intro ls
+      cases ls
+      · simp [List.mem, List.splits]
+      · simp [List.mem, List.splits]
+        apply List.memAppendLeft
+        apply List.mapMem
+        exact allSplits _
+
+/-
+Converts a `ListSplit` to the corresponding pair of lists created by the split.
+-/
+def ListSplit.toList {a : α} {l : List α}
+  : ListSplit a l → { listpair : List α × List α // l = listpair.fst ++ [a] ++ listpair.snd }
+  | head t => ⟨([], t), by simp⟩
+  | cons h ls =>
+    match ls.toList with
+      | ⟨(lsfst, lssnd), lsprf⟩ => ⟨(h :: lsfst, lssnd), by simp [lsprf]⟩
+
+/-
+A inductive definition of a split of a word into two words such that a conjugate of the first appended to the second gives the full word.
+-/
+inductive ConjugateSplit : Word α → Type _
+  | split : (l : Alphabet α) → (fstword : Word α) → (sndword : Word α) → ConjugateSplit (fstword^l ++ sndword)
+  deriving Repr
+
+def ListSplit.toConjugate {l : Alphabet α} {w : Word α} : ListSplit l⁻¹ w → ConjugateSplit (l :: w)
+  | ls =>
+    match ls.toList with
+      | ⟨(lsfst, lssnd), lsprf⟩ =>
+      let splitprf : l :: w = lsfst^l ++ lssnd := by simp [lsprf]
+      splitprf ▸ (ConjugateSplit.split l lsfst lssnd)
+
+def ConjugateSplit.toListSplit {l : Alphabet α} {w : Word α} : ConjugateSplit (l :: w) → ListSplit l⁻¹ w
+  | split _ fstword sndword =>
+    match fstword with
+      | [] => ListSplit.head _
+      | h :: t => ListSplit.cons _ (toListSplit (ConjugateSplit.split _ t sndword))
+
+
+theorem ListSplit.conjsplitid {l : Alphabet α} {w : Word α} (ls : ListSplit l⁻¹ w) : ls.toConjugate.toListSplit = ls := sorry
+theorem ConjugateSplit.conjsplitid {l : Alphabet α} {w : Word α} (cs : ConjugateSplit (l :: w)) : cs = cs.toListSplit.toConjugate := by
+  match cs with
+    | split _ fstword sndword =>
+      induction fstword with
+        | nil =>
+          simp [ConjugateSplit.toListSplit]
+          simp [ListSplit.toConjugate]
+          match (ListSplit.head (List.append [] sndword)).toList with
+            | ⟨(lsfst, lssnd), lsprf⟩ =>
+              sorry
+        | cons h t ih => sorry
+
+/-
+All conjugate splits of a word.
+-/
+def Word.conjugateSplits : (w : Word α) → List (ConjugateSplit w)
   | [] => []
-  | h :: tail =>
-    let tailSplits :=
-    (provedSplits l tail).map
-      (fun
-        | ⟨(fst, snd), prf⟩ =>
-          { val := (h :: fst, snd), property := by simp [prf] }
-      )
+  | l :: w' => (w'.splits l⁻¹).map (ListSplit.toConjugate)
 
-    if headmatch : h = l then
-      { val := ([], tail), property := by simp [headmatch] } :: tailSplits
-    else
-      tailSplits
+instance {w : Word α} : DecidableEq (ConjugateSplit w) := by
+  intro cs₁ cs₂; sorry
 
--- A split of the empty word cannot exist.
-@[simp] theorem splitEmpty {l : Alphabet α} : (ps : ProvedSplit l []) → False := by
-  intro ⟨(fst, snd), prf⟩
-  simp at prf
-  have emptyLenZero : List.length ([] : Word α) = Nat.zero := rfl
-  have splitLenPos : 0 < List.length (fst ++ [l] ++ snd) := by
-    simp
-    rw [Nat.add_assoc, Nat.add_comm, Nat.add_assoc, Nat.succ_add]
-    apply Nat.zero_lt_succ
-  have emptyLenPos : 0 < List.length ([] : Word α) := by
-    rw [prf]
-    exact splitLenPos
-  have zeroPos : Nat.zero < Nat.zero := emptyLenPos
-  apply Nat.lt_irrefl
-  exact zeroPos
+/-
+A proof that every possible split is contained in the output of `conjugateSplits`
+-/
+theorem ConjugateSplit.allSplits {w : Word α} : ∀ cs : ConjugateSplit w, cs ∈ w.conjugateSplits := by
+  match w with
+    | [] =>
+      intro cs
+      cases cs
+    | l :: w' =>
+      intro cs
+      simp [Word.conjugateSplits, List.mem]
+      rw [ConjugateSplit.conjsplitid cs]
+      apply List.mapMem
+      apply ListSplit.allSplits
 
--- A split is always smaller than the original word.
-@[simp] theorem splitBound {l : Alphabet α} : {w : Word α} → (ps : ProvedSplit l w) →
-(ps.val.fst.length + ps.val.snd.length < w.length) := by
-  intro w
-  induction w with
-    | nil =>
-    intro ps
-    apply False.elim
-    apply splitEmpty ps
-    | cons h w' =>
-    intro ⟨(fst, snd), prf⟩
-    simp [prf]
-    rw [Nat.add_comm _ (Nat.succ 0), Nat.add_assoc, Nat.succ_add, Nat.zero_add]
-    apply Nat.lt_succ_self
+/-
+@[simp] def ConjugateSplit.fstword {w : Word α} : ConjugateSplit w → Word α
+  | split _ fstword _ => fstword
 
--- The first part of the split is smaller than the entire word.
-@[simp] theorem fstSplitBound {l : Alphabet α} : (w : Word α) →
-(ps : ProvedSplit l w) → (ps.val.fst.length < w.length) := by
-  intro w; intro ⟨(fst, snd), prf⟩
-  simp [prf]
-  rw [Nat.add_assoc, Nat.succ_add]
-  apply Nat.lt_add_right
+@[simp] def ConjugateSplit.sndword {w : Word α} : ConjugateSplit w → Word α
+  | split _ _ sndword => sndword
 
--- The second part of the split is smaller than the entire word.
-@[simp] theorem sndSplitBound {l : Alphabet α} : (w : Word α) →
-(ps : ProvedSplit l w) → (ps.val.snd.length < w.length) := by
-  intro w ; intro ⟨(fst, snd), prf⟩
-  simp [prf]
-  rw [Nat.add_succ]
-  apply Nat.lt_add_left
+@[simp] theorem ConjugateSplit.fstwordLen {w : Word α} : (cs : ConjugateSplit w) → cs.fstword.length < w.length
+  | split l fst snd => by
+    simp; rw [BoundProof.conj]; simp
+    have : Nat.succ (fst.length + Nat.succ Nat.zero) = fst.length + (Nat.succ (Nat.succ Nat.zero)) := by simp
+    rw [this, Nat.add_assoc, Nat.succ_add]
+    apply Nat.lt_add_right
 
--- A bound on the first part of a split of a "cons" word, useful for showing termination.
-@[simp] theorem fstConsSplit {h : Alphabet α} {first second tail : Word α}
-  (prf : tail = (first, second).fst ++ [h⁻¹] ++ (first, second).snd)
-  : List.length first < List.length (h :: tail) := by
-   simp [prf]
-   rw [Nat.add_assoc, Nat.succ_add, Nat.zero_add]
-   apply Nat.lt_trans (Nat.lt_add_right _ _) (Nat.lt_succ_self _)
-
--- A bound on the second part of a split of a "cons" word, useful for showing termination.
-@[simp] theorem sndConsSplit {h : Alphabet α} {first second tail : Word α}
-  (prf : tail = (first, second).fst ++ [h⁻¹] ++ (first, second).snd)
-  : List.length second < List.length (h :: tail) := by
-   simp [prf]
-   rw [Nat.add_succ, Nat.add_zero]
-   apply Nat.lt_trans (Nat.lt_add_left _ _) (Nat.lt_succ_self _)
-
-end ProvedSplit
-
-/-decreasing_by {
-  -- source: https://github.com/leanprover/lean4/blob/de197675946ff37b1ae03c6bebe4ca58bb089fa9/tests/lean/run/wfrecUnary.lean
-  simp [measure, id, invImage, InvImage, Nat.lt_wfRel, WellFoundedRelation.rel, sizeOf] <;>
-
-  simp [Nat.lt_succ_self] <;>
-
-  (first
-    | apply (ProvedSplit.fstConsSplit prf)
-    | apply (ProvedSplit.sndConsSplit prf)
-    | assumption
-  )
-}
+@[simp] theorem ConjugateSplit.sndwordLen {w : Word α} : (cs : ConjugateSplit w) → cs.sndword.length < w.length
+  | split l fst snd => by
+    simp; apply Nat.lt_add_left
 -/
