Polylean/WatsonCrickLength.lean
@@ -5,18 +5,12 @@ A non-crossing match is inductively defined to be one of
 - the empty word
 - a letter of the alphabet attached to the front of a non-crossing match
 - a conjugate of a non-crossing match appended to the front of a non-crossing match
-
-Example:
-
-  .---------.
-    .--.
-α β α α⁻¹ β β⁻¹  ↦   α :: (matching β (matching α [] (β :: [])) [])
 -/
-inductive MatchWord (α : Type _) [DecidableEq α]
-  | nil : MatchWord α
-  | cons : Alphabet α → MatchWord α → MatchWord α
-  | matching : Alphabet α → MatchWord α → MatchWord α → MatchWord α
-  deriving Repr --, DecidableEq
+inductive MatchWord {α : Type _} [DecidableEq α] : Word α → Type _
+  | nil : MatchWord []
+  | cons {w' : Word α} : (l : Alphabet α) → MatchWord w' → MatchWord (l :: w')
+  | matching {fst snd : Word α} : (l : Alphabet α) → MatchWord fst → MatchWord snd → MatchWord (fst^l ++ snd)
+  deriving Repr
 
 
 namespace MatchWord
@@ -26,46 +20,55 @@ variable {α : Type _} [DecidableEq α]
 /-
 The number of un-matched letters in a matching.
 -/
-@[reducible, simp] def unmatchedCount : MatchWord α → ℕ
-  | nil => 0
-  | cons l w => 1 + unmatchedCount w
-  | matching _ w w' => unmatchedCount w + unmatchedCount w'
-
-/-
-Converts a non-crossing match word to the corresponding usual word.
--/
-@[reducible, simp] def toWord : MatchWord α → Word α
-  | nil => []
-  | cons l w => l :: (toWord w)
-  | matching l w w' => (toWord w)^l ++ (toWord w')
-
-
-/-
-Defining a "matching" corresponding to a word.
--/
-@[reducible] def isMatching (m : MatchWord α) (w : Word α) := m.toWord = w
-
-infix:100 " is a matching of " => MatchWord.isMatching
-
-abbrev Matching (w : Word α) := {m : MatchWord α // m is a matching of w}
-
+@[simp] def unmatchedCount : {w : Word α} → (MatchWord w) → ℕ
+  | _, nil              => Nat.zero
+  | _, cons _ m'        => Nat.succ (unmatchedCount m')
+  | _, matching _ m₁ m₂ => unmatchedCount m₁ + unmatchedCount m₂
 
 /-
 A total order on the matchings of a word in terms of the "energy" (the number of unmatched letters).
 -/
-instance {w : Word α} : LE (Matching w) :=
- ⟨λ m m' => unmatchedCount m.val ≤ unmatchedCount m'.val⟩
+instance {w : Word α} : LE (MatchWord w) :=
+ ⟨λ m m' => unmatchedCount m ≤ unmatchedCount m'⟩
 
-instance {w : Word α} : ∀ m m' : Matching w, Decidable (m ≤ m') := by
-  intro ; intro
-  simp [LE.le]; exact inferInstance
+instance {w : Word α} : ∀ m m' : MatchWord w, Decidable (m ≤ m') := by
+  intro ; intro ; simp [LE.le] ; exact inferInstance
 
+instance {w : Word α} : TotalOrder (MatchWord w) := {
+  reflLE := by { intro a; simp [LE.le] ; cases a <;> simp },
+  -- antisymmetry does not hold for `MatchWord`
+  transLE := by {intro a b c; simp [LE.le]; intro hab hbc; exact Nat.le_trans hab hbc}
+  totalLE := by {intro a b; simp [LE.le]; apply Nat.le_total}
+}
 
 /-
-The empty matching cannot correspond to a non-empty word.
+Takes a word `w` as input and returns a maximal matching
+(a matching with the lowest number of unmatched letters) of the word.
 -/
-theorem consNeEmptyMatch (l : Alphabet α) (w : Word α) : ¬(nil is a matching of (l :: w)) := by
-  intro h_match ; simp [isMatching] at h_match
+def maxMatch : (w : Word α) → MatchWord w
+  | List.nil => MatchWord.nil
+  | List.cons l w' =>
+    let base := MatchWord.cons l (maxMatch w')
+    let splits := (Word.conjugateSplits (l :: w')).map
+      ( fun
+          | ConjugateSplit.split l fst snd =>
+            matching l (maxMatch fst) (maxMatch snd) )
+    List.foldl min base splits
+termination_by _ w => List.length w
+decreasing_by {
+  -- source: https://github.com/leanprover/lean4/blob/de197675946ff37b1ae03c6bebe4ca58bb089fa9/tests/lean/run/wfrecUnary.lean
+  simp [measure, id, invImage, InvImage, Nat.lt_wfRel, WellFoundedRelation.rel, sizeOf] <;>
+  first
+    | rw [← Nat.add_succ, Nat.add_assoc]; apply Nat.lt_add_right
+    | rw [← Nat.succ_add]; apply Nat.lt_add_left
+}
+
+/-
+The definition of Watson-Crick length, as the number of unmatched letters in a minimal matching of the word.
+-/
+def WatsonCrickLength : FreeGroupLength α :=
+  λ w => unmatchedCount $ maxMatch w
+
 
 /-
 If `m` is a matching of a word `w`, the length of `w` under any pseudo-length function is
@@ -73,16 +76,16 @@ bounded by the "energy" of `m` (the number of unmatched letters).
 
 This theorem is crucial for proving the maximality of the Watson-Crick length.
 -/
-theorem unmatchedCountBound (m : MatchWord α)
-  : (m.toWord is bounded by m.unmatchedCount) := by
+theorem unmatchedCountBound {w : Word α} (m : MatchWord w) :
+  (w is bounded by m.unmatchedCount) := by
   induction m with
     | nil =>
       intro ; intro
       simp [PseudoLengthFunction.emptyWord]
     | cons =>
       intro ; intro
-      apply BoundProof.prepend
-      assumption
+      simp ; rw [Nat.succ_eq_one_add]
+      apply BoundProof.prepend ; assumption
     | matching =>
       intro ; intro
       apply BoundProof.triangIneq
@@ -90,40 +93,11 @@ theorem unmatchedCountBound (m : MatchWord α)
       · assumption
 
 /-
-Takes a word `w` as input and returns a maximal matching
-(a matching with the lowest number of unmatched letters) of the word.
+A proof that the output of `maxMatch` has the least number of unmatched letters among all possible matchings of a word.
 -/
-def maxMatch : (w : Word α) → Matching w
-  | List.nil => ⟨MatchWord.nil, rfl⟩  -- the trivial case of the empty word
-  | List.cons l w' =>
+theorem maximalMatching {w : Word α} : (m : MatchWord w) → (maxMatch w) ≤ m
+  | nil => sorry
+  | cons l m' => sorry
+  | matching l m₁ m₂ => sorry
 
-    -- the case where the first letter is unmatched
-    let base : Matching (l :: w') :=
-      let ⟨w'Match, w'Prf⟩ := maxMatch w'
-      ⟨MatchWord.cons l w'Match, by simp [w'Prf]⟩
-
-    -- the case where the first letter is matched
-    let splits : List (Matching (l :: w')) :=
-    (ProvedSplit.provedSplits l⁻¹ w').map (λ ⟨⟨fst, snd⟩, prf⟩ =>
-          -- proof that the length of the word decreases, required for showing termination
-          have : fst.length < (l :: w').length := ProvedSplit.fstConsSplit prf
-          let ⟨fstMatch, fstPrf⟩ := maxMatch fst -- a maximal matching of the first part of the split
-
-          -- proof that the length of the word decreases, required for showing termination
-          have : snd.length < (l :: w').length := ProvedSplit.sndConsSplit prf
-          let ⟨sndMatch, sndPrf⟩ := maxMatch snd -- a maximal matching of the second part of the split
-
-          {
-            -- creates a matching involving the first letter of the word
-            val := (MatchWord.matching l fstMatch sndMatch),
-            property := by
-             rw [prf, BoundProof.conjSplit, ← fstPrf, ← sndPrf]
-          }
-      )
-
-    -- the best matching of the ones above, i.e., the one with the least unmatched letters ("energy")
-    splits.foldl min base
-
-termination_by _ w => List.length w -- this function terminates since the length of the input list decreases on each recursive call
-
-namespace MatchWord
+end MatchWord
