Polylean/Misc.lean
@@ -1,0 +1,158 @@
+/-
+Miscellaneous theorems on natural numbers.
+-/
+namespace Nat
+
+attribute [simp] Nat.le_refl
+attribute [simp] Nat.lt_succ_self
+
+protected theorem le_shift_left {a b c : Nat} : a ≤ b → c + a ≤ c + b := by
+  intro h
+  induction c with
+  | zero => simp [h]
+  | succ _ ih => simp [Nat.succ_add, Nat.succ_le_succ ih]
+
+protected theorem le_shift_right {a b c : Nat} : a ≤ b → a + c ≤ b + c := by
+  intro h
+  induction c with
+    | zero => simp [h]
+    | succ _ ih => simp [Nat.add_succ, Nat.succ_le_succ ih]
+
+protected theorem succ_eq_one_add : ∀ m : Nat, Nat.succ m = (Nat.succ Nat.zero) + m :=
+  λ m => by simp [Nat.succ_add]
+
+protected theorem lt_add_right : ∀ m n : Nat, m < m + (Nat.succ n) := by
+  intro m n
+  induction n with
+  | zero =>
+    rw [Nat.add_succ, Nat.add_zero]
+    apply Nat.lt_succ_self
+  | succ n ih =>
+    rw [Nat.add_succ]
+    apply Nat.lt_trans ih (Nat.lt_succ_self _)
+
+protected theorem lt_add_left : ∀ m n : Nat, m < Nat.succ n + m := by
+  intro m n
+  induction n with
+    | zero =>
+      rw [Nat.succ_add, Nat.zero_add]
+      apply Nat.lt_succ_self
+    | succ n ih =>
+      rw [Nat.succ_add]
+      apply Nat.lt_trans ih (Nat.lt_succ_self _)
+
+end Nat
+
+class TotalOrder (α : Type _) [LE α] [DecidableRel (@LE.le α _)] where
+  (reflLE : ∀ a : α, a ≤ a)
+--  (antisymmLE : ∀ {a b : α}, a ≤ b → b ≤ a → a = b) -- this is not strictly necessary for the proofs
+  (transLE : ∀ {a b c : α}, a ≤ b → b ≤ c → a ≤ c)
+  (totalLE : ∀ a b : α, a ≤ b ∨ b ≤ a)
+
+open TotalOrder
+
+variable {α : Type _} [LE α] [DecidableRel (@LE.le α _)] [∀ a b : α, Decidable (a = b)] [TotalOrder α]
+variable {β : Type _} [LE β] [DecidableRel (@LE.le β _)] [∀ a b : β, Decidable (a = b)] [TotalOrder β]
+
+@[simp] theorem minFst (a b : α) : min a b ≤ a :=
+  if h:a ≤ b then by
+    simp [min, h, reflLE]
+  else by
+    simp [min, h]
+    match (totalLE a b) with
+      | Or.inl _ => apply False.elim; apply h; assumption
+      | Or.inr _ => assumption
+
+@[simp] theorem minSnd (a b : α) : min a b ≤ b :=
+  if h:a ≤ b then by
+    simp [min, h]
+  else by
+    simp [min, h, reflLE]
+
+namespace List
+
+theorem foldMinBase (b : α) : (as : List α) → foldl min b as ≤ b
+  | [] => reflLE _
+  | h :: tail => transLE (foldMinBase (min b h) tail) (minFst _ _)
+
+def mem (a : α) : List α → Bool
+  | [] => false
+  | h :: tail => if (h = a) then true else mem a tail
+
+infix:100 " ∈ " => mem
+
+theorem foldMinMem (a b : α) (as : List α) (amember : a ∈ as) : foldl min b as ≤ a :=
+  match as with
+    | [] => by
+      apply False.elim
+      simp [mem] at amember
+    | h :: tail =>
+      if headmatch:(h = a) then by
+        simp [*, headmatch, foldl, mem] at *
+        apply transLE
+        exact foldMinBase _ tail
+        simp
+      else by
+        simp [*, headmatch, foldl, mem] at *
+        exact foldMinMem a _ tail amember
+
+theorem mapMem (f : α → β) {a : α} {l : List α} (amember : a ∈ l) :
+  (f a) ∈ (map f l) := by
+  induction l with
+    | nil =>
+      apply False.elim
+      simp [mem] at amember
+    | cons h t ih =>
+      simp [map, mem] at *
+      exact if headmatch:h = a then by
+        simp [congrArg f headmatch]
+      else by
+        simp [headmatch] at amember
+        simp [amember] at ih
+        exact if fheadmatch:(f h = f a) then by
+          simp [fheadmatch]
+        else by
+          simp [fheadmatch, ih]
+
+theorem memAppendLeft {a : α} {l₁ l₂ : List α} :
+  a ∈ l₂ → a ∈ (l₁ ++ l₂) := by
+  induction l₁ with
+  | nil =>
+    simp
+    exact id
+  | cons h t ih =>
+    simp [mem]
+    exact if headmatch:(h = a) then by
+      simp [headmatch]
+    else by
+      simp [headmatch]
+      exact ih
+
+theorem memAppendRight {a : α} {l₁ l₂ : List α} :
+  a ∈ l₁ → a ∈ (l₁ ++ l₂) := by
+  induction l₁ with
+  | nil =>
+    intro hyp
+    simp [mem] at hyp
+  | cons h t ih =>
+    simp [mem]
+    exact if headmatch:(h = a) then by
+      simp [headmatch]
+    else by
+      simp [headmatch]
+      exact ih
+
+@[simp] theorem appendLength {α : Type _} {l₁ l₂ : List α} :
+  List.length (List.append l₁ l₂) = l₁.length + l₂.length := by
+  show (List.length (l₁ ++ l₂)) = l₁.length + l₂.length
+  simp
+
+end List
+
+instance : TotalOrder Nat :=
+  {
+    reflLE := Nat.le_refl,
+--    antisymmLE := Nat.le_antisymm,
+    transLE := Nat.le_trans,
+    totalLE := Nat.le_total
+  }
